support riscv loads and stores

examples/riscv64_test.s
@@ -1,6 +1,8 @@
 test:
     mv      a0, zero
     addi    a0, a0, 1
+    sd      a1, 8(sp)
+    ld      a1, 8(sp)
     beq     a0, a1, .END
     nop
 .END:
