examples/riscv64_test.v
@@ -1,24 +1,27 @@
 Require Import isla.riscv64.riscv64.
 From isla.instructions.riscv64_test Require Import instrs.
 
-Definition misa_bits : bv 64 :=
-  [BV{64}0x800000000015312d].
-
 Definition riscv_test_spec (x11 : bv 64) : spec :=
   (sif (bv_unsigned x11 = 1)
-               (scons (SInstrTrap [BV{64} 0x0000000010300010]) snil)
-               (scons (SInstrTrap [BV{64} 0x000000001030000c]) snil)).
+               (scons (SInstrTrap [BV{64} 0x0000000010300018]) snil)
+               (scons (SInstrTrap [BV{64} 0x0000000010300014]) snil)).
 
-Lemma riscv_test `{!islaG Σ} `{!threadG} (x11 : bv 64):
+Lemma riscv_test `{!islaG Σ} `{!threadG} (x2 x11 : bv 64):
   instr 0x0000000010300000 (Some a0) -∗
   instr 0x0000000010300004 (Some a4) -∗
   instr 0x0000000010300008 (Some a8) -∗
-  instr 0x000000001030000c None -∗
-  instr 0x0000000010300010 None -∗
+  instr 0x000000001030000c (Some ac) -∗
+  instr 0x0000000010300010 (Some a10) -∗
+  instr 0x0000000010300014 None -∗
+  instr 0x0000000010300018 None -∗
   instr_body 0x0000000010300000 (
+    reg_col sys_regs ∗
     "x10" ↦ᵣ: λ _,
+    "x2" ↦ᵣ RVal_Bits x2 ∗
     "x11" ↦ᵣ RVal_Bits x11 ∗
-    "misa" ↦ᵣ RegVal_Struct [("bits", RVal_Bits misa_bits)] ∗
+    ⌜bv_unsigned x2 `mod` 8 = 0⌝ ∗
+    ⌜0x0000000080000000 ≤ bv_unsigned x2 + 8 < 0x0000000080000000 + 0x0000000004000000⌝ ∗
+    bv_add_Z x2 8 ↦ₘ? 8 ∗
     spec_trace (riscv_test_spec x11) ∗
     True
   ).
@@ -30,37 +33,66 @@ Proof.
   - rewrite /riscv_test_spec sif_true //.
 Qed.
 
-Definition riscv_test_regs (x10 x11 : bv 64) : reg_map :=
+Definition riscv_test_regs (mstatus_bits satp x2 x10 x11 : bv 64) : reg_map :=
     <[ "PC" := RVal_Bits [BV{64} 0x0000000010300000] ]> $
+    <[ "x2" := RVal_Bits x2 ]> $
     <[ "x10" := RVal_Bits x10 ]> $
     <[ "x11" := RVal_Bits x11 ]> $
-    <[ "misa" := RegVal_Struct [("bits", RVal_Bits misa_bits)] ]> $
-    ∅.
+    sys_regs_map mstatus_bits satp.
 
-Definition riscv_test_state_global := {|
+Definition riscv_test_state_global (x2 : bv 64) := {|
     seq_instrs :=
     <[ [BV{64} 0x0000000010300000] := a0]> $
     <[ [BV{64} 0x0000000010300004] := a4]> $
     <[ [BV{64} 0x0000000010300008] := a8]> $
+    <[ [BV{64} 0x000000001030000c] := ac]> $
+    <[ [BV{64} 0x0000000010300010] := a10]> $
     ∅;
-    seq_mem := ∅
+    seq_mem := list_to_map (zip (bv_seq (bv_add_Z x2 8) 8) (replicate 8 (bv_0 8)))
 |}.
+Local Arguments zip_with : simpl never.
+Local Arguments list_to_map : simpl never.
 
-Lemma riscv_test_adequate x10 x11 κs n t2 σ2:
-  nsteps n (initial_local_state <$> [riscv_test_regs x10 x11],
-            riscv_test_state_global) κs (t2, σ2) →
+Lemma riscv_test_adequate mstatus_bits satp x2 x10 x11 κs n t2 σ2:
+  bv_extract 17 1 mstatus_bits = [BV{1} 0] →
+  bv_unsigned x2 `mod` 8 = 0 →
+  0x0000000080000000 ≤ bv_unsigned x2 + 8 < 0x0000000080000000 + 0x0000000004000000 →
+  nsteps n (initial_local_state <$> [riscv_test_regs mstatus_bits satp x2 x10 x11],
+            riscv_test_state_global x2) κs (t2, σ2) →
   (∀ e2, e2 ∈ t2 → not_stuck e2 σ2) ∧ riscv_test_spec x11 κs.
 Proof.
+  move => ???.
   set Σ : gFunctors := #[islaΣ].
   apply: (isla_adequacy Σ) => //.
   { unfold riscv_test_spec. destruct (decide ((bv_unsigned x11 = 1))); spec_solver. }
-  iIntros (?) "#Hi #Hbm Hspec /= !>". iSplitL => //.
-  iIntros (?).
+  iIntros (?) "#Hi #Hbm Hspec Hmem /= !>". iSplitL => //. iIntros (?).
+  iAssert (bv_add_Z x2 8 ↦ₘ? 8)%I with "[Hmem]" as "?". {
+    rewrite big_sepM_list_to_map. 2: { rewrite fst_zip //. by apply NoDup_bv_seq. }
+    rewrite /zip_with/=.
+    iDestruct "Hmem" as "(Hm1&Hm2&Hm3&Hm4&Hm5&Hm6&Hm7&Hm8&_)".
+    rewrite bv_add_Z_0.
+    iApply (mem_mapsto_uninit_combine 1 with "[Hm1]"); [done|by iApply (mem_mapsto_mapsto_to_uninit _ _ 8)|].
+    iApply (mem_mapsto_uninit_combine 1 with "[Hm2]"); [done|by iApply (mem_mapsto_mapsto_to_uninit _ _ 8)|].
+    rewrite -(bv_add_Z_add_r _ 1 1).
+    iApply (mem_mapsto_uninit_combine 1 with "[Hm3]"); [done|by iApply (mem_mapsto_mapsto_to_uninit _ _ 8)|].
+    rewrite -(bv_add_Z_add_r _ 1 _).
+    iApply (mem_mapsto_uninit_combine 1 with "[Hm4]"); [done|by iApply (mem_mapsto_mapsto_to_uninit _ _ 8)|].
+    rewrite -(bv_add_Z_add_r _ 1 _).
+    iApply (mem_mapsto_uninit_combine 1 with "[Hm5]"); [done|by iApply (mem_mapsto_mapsto_to_uninit _ _ 8)|].
+    rewrite -(bv_add_Z_add_r _ 1 _).
+    iApply (mem_mapsto_uninit_combine 1 with "[Hm6]"); [done|by iApply (mem_mapsto_mapsto_to_uninit _ _ 8)|].
+    rewrite -(bv_add_Z_add_r _ 1 _).
+    iApply (mem_mapsto_uninit_combine 1 with "[Hm7]"); [done|by iApply (mem_mapsto_mapsto_to_uninit _ _ 8)|].
+    rewrite -(bv_add_Z_add_r _ 1 _).
+    iApply (mem_mapsto_uninit_combine 1 with "[Hm8]"); [done|by iApply (mem_mapsto_mapsto_to_uninit _ _ 8)|].
+    by rewrite mem_mapsto_uninit_0.
+  }
   do 4 (rewrite big_sepM_insert; [|by vm_compute]).
-  iIntros "(?&?&?&?&?)".
-  iApply wp_asm_thread_ctx. iIntros (?) "Hctx". iModIntro. iFrame.
+  iIntros "(?&?&?&?&Hsys)".
+  iApply wp_asm_thread_ctx. iIntros (?) "Hctx".
+  iMod (sys_regs_init with "Hctx Hsys") as "[$ Hsys]"; [done|]. iModIntro.
   iApply (wp_next_instr_pre with "[$] []").
-  - iApply (riscv_test x11).
+  - iApply (riscv_test x2 x11).
     all: try by unshelve iApply (instr_intro with "Hi").
   - repeat liAStep.
 Qed.
