instructions/riscv64_test/a10.v
@@ -1,0 +1,39 @@
+From isla Require Import isla_lang.
+
+Definition a10 : list trc := [
+  [
+    Smt (DeclareConst 0%Z (Ty_BitVec 64%N)) Mk_annot;
+    Assume (AExp_Binop (Eq) (AExp_Unop (Extract 1%N 1%N) (AExp_Val (AVal_Var "PC" []) Mk_annot) Mk_annot) (AExp_Val (AVal_Bits [BV{1%N} 0x0%Z]) Mk_annot) Mk_annot) Mk_annot;
+    Smt (Assert (Binop (Eq) (Unop (Extract 1%N 1%N) (Val (Val_Symbolic 0%Z) Mk_annot) Mk_annot) (Val (Val_Bits [BV{1%N} 0x0%Z]) Mk_annot) Mk_annot)) Mk_annot;
+    ReadReg "PC" [] (RegVal_Base (Val_Symbolic 0%Z)) Mk_annot;
+    Smt (DefineConst 1%Z (Manyop (Bvmanyarith Bvadd) [Val (Val_Symbolic 0%Z) Mk_annot; Val (Val_Bits [BV{64%N} 0x4%Z]) Mk_annot] Mk_annot)) Mk_annot;
+    Smt (DeclareConst 13%Z (Ty_BitVec 64%N)) Mk_annot;
+    ReadReg "x10" [] (RegVal_Base (Val_Symbolic 13%Z)) Mk_annot;
+    Smt (DeclareConst 14%Z (Ty_BitVec 64%N)) Mk_annot;
+    ReadReg "x11" [] (RegVal_Base (Val_Symbolic 14%Z)) Mk_annot;
+    Smt (DefineConst 15%Z (Binop (Eq) (Val (Val_Symbolic 13%Z) Mk_annot) (Val (Val_Symbolic 14%Z) Mk_annot) Mk_annot)) Mk_annot;
+    Branch 0%Z "model/riscv_insts_base.sail 186:2 - 204:23" Mk_annot;
+    Smt (Assert (Unop (Not) (Val (Val_Symbolic 15%Z) Mk_annot) Mk_annot)) Mk_annot;
+    WriteReg "PC" [] (RegVal_Base (Val_Symbolic 1%Z)) Mk_annot
+  ];
+  [
+    Smt (DeclareConst 0%Z (Ty_BitVec 64%N)) Mk_annot;
+    Assume (AExp_Binop (Eq) (AExp_Unop (Extract 1%N 1%N) (AExp_Val (AVal_Var "PC" []) Mk_annot) Mk_annot) (AExp_Val (AVal_Bits [BV{1%N} 0x0%Z]) Mk_annot) Mk_annot) Mk_annot;
+    Smt (Assert (Binop (Eq) (Unop (Extract 1%N 1%N) (Val (Val_Symbolic 0%Z) Mk_annot) Mk_annot) (Val (Val_Bits [BV{1%N} 0x0%Z]) Mk_annot) Mk_annot)) Mk_annot;
+    ReadReg "PC" [] (RegVal_Base (Val_Symbolic 0%Z)) Mk_annot;
+    Smt (DefineConst 1%Z (Manyop (Bvmanyarith Bvadd) [Val (Val_Symbolic 0%Z) Mk_annot; Val (Val_Bits [BV{64%N} 0x4%Z]) Mk_annot] Mk_annot)) Mk_annot;
+    Smt (DeclareConst 13%Z (Ty_BitVec 64%N)) Mk_annot;
+    ReadReg "x10" [] (RegVal_Base (Val_Symbolic 13%Z)) Mk_annot;
+    Smt (DeclareConst 14%Z (Ty_BitVec 64%N)) Mk_annot;
+    ReadReg "x11" [] (RegVal_Base (Val_Symbolic 14%Z)) Mk_annot;
+    Smt (DefineConst 15%Z (Binop (Eq) (Val (Val_Symbolic 13%Z) Mk_annot) (Val (Val_Symbolic 14%Z) Mk_annot) Mk_annot)) Mk_annot;
+    Smt (DefineConst 16%Z (Manyop (Bvmanyarith Bvadd) [Val (Val_Symbolic 0%Z) Mk_annot; Val (Val_Bits [BV{64%N} 0x8%Z]) Mk_annot] Mk_annot)) Mk_annot;
+    Branch 0%Z "model/riscv_insts_base.sail 186:2 - 204:23" Mk_annot;
+    Smt (Assert (Val (Val_Symbolic 15%Z) Mk_annot)) Mk_annot;
+    Smt (DefineConst 17%Z (Unop (Extract 0%N 0%N) (Binop ((Bvarith Bvlshr)) (Val (Val_Symbolic 16%Z) Mk_annot) (Val (Val_Bits [BV{64%N} 0x1%Z]) Mk_annot) Mk_annot) Mk_annot)) Mk_annot;
+    Smt (Assert (Unop (Not) (Binop (Eq) (Val (Val_Symbolic 17%Z) Mk_annot) (Val (Val_Bits [BV{1%N} 0x1%Z]) Mk_annot) Mk_annot) Mk_annot)) Mk_annot;
+    Smt (Assert (Unop (Not) (Unop (Not) (Binop (Eq) (Val (Val_Symbolic 17%Z) Mk_annot) (Val (Val_Bits [BV{1%N} 0x0%Z]) Mk_annot) Mk_annot) Mk_annot) Mk_annot)) Mk_annot;
+    BranchAddress (RegVal_Base (Val_Symbolic 16%Z)) Mk_annot;
+    WriteReg "PC" [] (RegVal_Base (Val_Symbolic 16%Z)) Mk_annot
+  ]
+].
