instructions/riscv64_test/ac_spec.v
@@ -1,0 +1,18 @@
+Require Import isla.isla.
+Require Import isla.riscv64.riscv64.
+Require Export isla.instructions.riscv64_test.ac.
+
+Lemma ac_spec `{!islaG Σ} `{!threadG}:
+  instr 0x1030000c (Some ac) -∗
+  instr_body 0x1030000c (ld_spec 0x000000001030000c "x11" "x2" (8)).
+Proof.
+  iStartProof.
+  repeat liAStep; liShow.
+
+  Unshelve. all: prepare_sidecond.
+  all: bv_solve.
+Qed.
+
+Definition ac_spec_inst `{!islaG Σ} `{!threadG} :=
+  entails_to_simplify_hyp 0 ac_spec.
+Global Existing Instance ac_spec_inst.
