instructions/riscv64_test/instrs.v
@@ -2,9 +2,15 @@ Require Import isla.isla_lang.
 Require Export isla.instructions.riscv64_test.a0.
 Require Export isla.instructions.riscv64_test.a4.
 Require Export isla.instructions.riscv64_test.a8.
+Require Export isla.instructions.riscv64_test.a8_spec.
+Require Export isla.instructions.riscv64_test.ac.
+Require Export isla.instructions.riscv64_test.ac_spec.
+Require Export isla.instructions.riscv64_test.a10.
 
 Definition instr_map := [
   (0x0%Z, a0 (* li a0,0 *));
   (0x4%Z, a4 (* addi a0,a0,1 *));
-  (0x8%Z, a8 (* beq a0,a1,10 <.END> *))
+  (0x8%Z, a8 (* sd a1,8(sp) *));
+  (0xc%Z, ac (* ld a1,8(sp) *));
+  (0x10%Z, a10 (* beq a0,a1,18 <.END> *))
 ].
