theories/riscv64/riscv64.v
@@ -1,2 +1,2 @@
 Require Export isla.isla.
-From isla.riscv64 Require Export arch.
+From isla.riscv64 Require Export arch sys_regs specs.
