theories/riscv64/specs.v
@@ -1,0 +1,37 @@
+Require Import isla.automation.
+Require Import isla.riscv64.arch.
+Require Import isla.riscv64.sys_regs.
+
+Definition sd_spec `{!islaG Σ} `{!threadG} (pc : Z) (R1 R2 : string) (offset : Z) : iProp Σ :=
+  ∃ (r1 r2 : bv 64),
+  reg_col sys_regs ∗
+  R1 ↦ᵣ RVal_Bits r1 ∗
+  R2 ↦ᵣ RVal_Bits r2 ∗
+  (bv_add_Z r2 offset) ↦ₘ? 8 ∗
+  ⌜bv_unsigned r2 `mod` 8 = 0⌝ ∗
+  ⌜0x0000000080000000 ≤ bv_unsigned r2 + offset < 0x0000000080000000 + 0x0000000004000000⌝ ∗
+  instr_pre (pc + 4) (
+    reg_col sys_regs ∗
+    R1 ↦ᵣ RVal_Bits r1 ∗
+    R2 ↦ᵣ RVal_Bits r2 ∗
+    (bv_add_Z r2 offset) ↦ₘ r1 ∗
+    True
+  ).
+Global Instance : LithiumUnfold (@sd_spec) := I.
+
+Definition ld_spec `{!islaG Σ} `{!threadG} (pc : Z) (R1 R2 : string) (offset : Z) : iProp Σ :=
+  ∃ (r1 r2 : bv 64),
+  reg_col sys_regs ∗
+  R1 ↦ᵣ: λ _,
+  R2 ↦ᵣ RVal_Bits r2 ∗
+  (bv_add_Z r2 offset) ↦ₘ r1 ∗
+  ⌜bv_unsigned r2 `mod` 8 = 0⌝ ∗
+  ⌜0x0000000080000000 ≤ bv_unsigned r2 + offset < 0x0000000080000000 + 0x0000000004000000⌝ ∗
+  instr_pre (pc + 4) (
+    reg_col sys_regs ∗
+    R1 ↦ᵣ RVal_Bits r1 ∗
+    R2 ↦ᵣ RVal_Bits r2 ∗
+    (bv_add_Z r2 offset) ↦ₘ r1 ∗
+    True
+  ).
+Global Instance : LithiumUnfold (@ld_spec) := I.
